Refactoring

OCL_Normal_Form.thy
@@ -61,80 +61,80 @@ inductive normalize
  LiteralN:
   "\<Gamma> \<turnstile> Literal a \<Rrightarrow> Literal a"
 |LetN:
-  "\<Gamma> \<turnstile> init1 \<Rrightarrow> init2 \<Longrightarrow>
-   \<Gamma>(v \<mapsto>\<^sub>f \<tau>) \<turnstile> body1 \<Rrightarrow> body2 \<Longrightarrow>
-   \<Gamma> \<turnstile> Let v \<tau> init1 body1 \<Rrightarrow> Let v \<tau> init2 body2"
+  "\<Gamma> \<turnstile> init\<^sub>1 \<Rrightarrow> init\<^sub>2 \<Longrightarrow>
+   \<Gamma>(v \<mapsto>\<^sub>f \<tau>) \<turnstile> body\<^sub>1 \<Rrightarrow> body\<^sub>2 \<Longrightarrow>
+   \<Gamma> \<turnstile> Let v \<tau> init\<^sub>1 body\<^sub>1 \<Rrightarrow> Let v \<tau> init\<^sub>2 body\<^sub>2"
 |VarN:
   "\<Gamma> \<turnstile> Var v \<Rrightarrow> Var v"
 |IfN:
-  "\<Gamma> \<turnstile> a1 \<Rrightarrow> a2 \<Longrightarrow>
-   \<Gamma> \<turnstile> b1 \<Rrightarrow> b2 \<Longrightarrow>
-   \<Gamma> \<turnstile> c1 \<Rrightarrow> c2 \<Longrightarrow>
-   \<Gamma> \<turnstile> If a1 b1 c1 \<Rrightarrow> If a2 b2 c2"
+  "\<Gamma> \<turnstile> a\<^sub>1 \<Rrightarrow> a\<^sub>2 \<Longrightarrow>
+   \<Gamma> \<turnstile> b\<^sub>1 \<Rrightarrow> b\<^sub>2 \<Longrightarrow>
+   \<Gamma> \<turnstile> c\<^sub>1 \<Rrightarrow> c\<^sub>2 \<Longrightarrow>
+   \<Gamma> \<turnstile> If a\<^sub>1 b\<^sub>1 c\<^sub>1 \<Rrightarrow> If a\<^sub>2 b\<^sub>2 c\<^sub>2"
 
 |MetaOperationCallN:
   "\<Gamma> \<turnstile> MetaOperationCall \<tau> op \<Rrightarrow> MetaOperationCall \<tau> op"
 |StaticOperationCallN:
-  "\<Gamma> \<turnstile>\<^sub>L as \<Rrightarrow> bs \<Longrightarrow>
-   \<Gamma> \<turnstile> StaticOperationCall \<tau> op as \<Rrightarrow> StaticOperationCall \<tau> op bs"
+  "\<Gamma> \<turnstile>\<^sub>L params\<^sub>1 \<Rrightarrow> params\<^sub>2 \<Longrightarrow>
+   \<Gamma> \<turnstile> StaticOperationCall \<tau> op params\<^sub>1 \<Rrightarrow> StaticOperationCall \<tau> op params\<^sub>2"
 
 |OclAnyDotCallN:
-  "\<Gamma> \<turnstile> src1 \<Rrightarrow> src2 \<Longrightarrow>
-   \<Gamma> \<turnstile> src2 : \<tau> \<Longrightarrow>
+  "\<Gamma> \<turnstile> src\<^sub>1 \<Rrightarrow> src\<^sub>2 \<Longrightarrow>
+   \<Gamma> \<turnstile> src\<^sub>2 : \<tau> \<Longrightarrow>
    \<tau> \<le> OclAny[1] \<or> \<tau> \<le> Tuple fmempty \<Longrightarrow>
-   (\<Gamma>, \<tau>) \<turnstile>\<^sub>C call1 \<Rrightarrow> call2 \<Longrightarrow>
-   \<Gamma> \<turnstile> Call src1 DotCall call1 \<Rrightarrow> Call src2 DotCall call2"
+   (\<Gamma>, \<tau>) \<turnstile>\<^sub>C call\<^sub>1 \<Rrightarrow> call\<^sub>2 \<Longrightarrow>
+   \<Gamma> \<turnstile> Call src\<^sub>1 DotCall call\<^sub>1 \<Rrightarrow> Call src\<^sub>2 DotCall call\<^sub>2"
 |OclAnySafeDotCallN:
-  "\<Gamma> \<turnstile> src1 \<Rrightarrow> src2 \<Longrightarrow>
-   \<Gamma> \<turnstile> src2 : \<tau> \<Longrightarrow>
+  "\<Gamma> \<turnstile> src\<^sub>1 \<Rrightarrow> src\<^sub>2 \<Longrightarrow>
+   \<Gamma> \<turnstile> src\<^sub>2 : \<tau> \<Longrightarrow>
    OclVoid[?] \<le> \<tau> \<Longrightarrow>
-   (\<Gamma>, \<tau>) \<turnstile>\<^sub>C call1 \<Rrightarrow> call2 \<Longrightarrow>
-   \<Gamma> \<turnstile> Call src1 SafeDotCall call1 \<Rrightarrow>
-       If (OperationCall src2 DotCall NotEqualOp [NullLiteral])
-          (Call src2 DotCall call2)
+   (\<Gamma>, \<tau>) \<turnstile>\<^sub>C call\<^sub>1 \<Rrightarrow> call\<^sub>2 \<Longrightarrow>
+   \<Gamma> \<turnstile> Call src\<^sub>1 SafeDotCall call\<^sub>1 \<Rrightarrow>
+       If (OperationCall src\<^sub>2 DotCall NotEqualOp [NullLiteral])
+          (Call src\<^sub>2 DotCall call\<^sub>2)
           NullLiteral"
 |OclAnyArrowDotCallN:
-  "\<Gamma> \<turnstile> src1 \<Rrightarrow> src2 \<Longrightarrow>
-   \<Gamma> \<turnstile> src2 : \<tau> \<Longrightarrow>
+  "\<Gamma> \<turnstile> src\<^sub>1 \<Rrightarrow> src\<^sub>2 \<Longrightarrow>
+   \<Gamma> \<turnstile> src\<^sub>2 : \<tau> \<Longrightarrow>
    \<tau> \<le> OclAny[?] \<or> \<tau> \<le> Tuple fmempty \<Longrightarrow>
-   (\<Gamma>, \<tau>) \<turnstile>\<^sub>C call1 \<Rrightarrow> call2 \<Longrightarrow>
-   \<Gamma> \<turnstile> Call src1 ArrowCall call1 \<Rrightarrow>
-       Call (OperationCall src2 DotCall OclAsSetOp []) ArrowCall call2"
+   (\<Gamma>, \<tau>) \<turnstile>\<^sub>C call\<^sub>1 \<Rrightarrow> call\<^sub>2 \<Longrightarrow>
+   \<Gamma> \<turnstile> Call src\<^sub>1 ArrowCall call\<^sub>1 \<Rrightarrow>
+       Call (OperationCall src\<^sub>2 DotCall OclAsSetOp []) ArrowCall call\<^sub>2"
 
 |CollectionArrowCallN:
-  "\<Gamma> \<turnstile> src1 \<Rrightarrow> src2 \<Longrightarrow>
-   \<Gamma> \<turnstile> src2 : \<tau> \<Longrightarrow>
+  "\<Gamma> \<turnstile> src\<^sub>1 \<Rrightarrow> src\<^sub>2 \<Longrightarrow>
+   \<Gamma> \<turnstile> src\<^sub>2 : \<tau> \<Longrightarrow>
    element_type \<tau> _ \<Longrightarrow>
-   (\<Gamma>, \<tau>) \<turnstile>\<^sub>C call1 \<Rrightarrow> call2 \<Longrightarrow>
-   \<Gamma> \<turnstile> Call src1 ArrowCall call1 \<Rrightarrow> Call src2 ArrowCall call2"
+   (\<Gamma>, \<tau>) \<turnstile>\<^sub>C call\<^sub>1 \<Rrightarrow> call\<^sub>2 \<Longrightarrow>
+   \<Gamma> \<turnstile> Call src\<^sub>1 ArrowCall call\<^sub>1 \<Rrightarrow> Call src\<^sub>2 ArrowCall call\<^sub>2"
 |CollectionSafeArrowCallN:
-  "\<Gamma> \<turnstile> src1 \<Rrightarrow> src2 \<Longrightarrow>
-   \<Gamma> \<turnstile> src2 : \<tau> \<Longrightarrow>
+  "\<Gamma> \<turnstile> src\<^sub>1 \<Rrightarrow> src\<^sub>2 \<Longrightarrow>
+   \<Gamma> \<turnstile> src\<^sub>2 : \<tau> \<Longrightarrow>
    element_type \<tau> \<sigma> \<Longrightarrow>
    OclVoid[?] \<le> \<sigma> \<Longrightarrow>
-   (\<Gamma>, \<tau>) \<turnstile>\<^sub>C call1 \<Rrightarrow> call2 \<Longrightarrow>
-   \<Gamma> \<turnstile> Call src1 SafeArrowCall call1 \<Rrightarrow>
-    Call (OperationCall src2 ArrowCall ExcludingOp [NullLiteral])
-      ArrowCall call2"
+   (\<Gamma>, \<tau>) \<turnstile>\<^sub>C call\<^sub>1 \<Rrightarrow> call\<^sub>2 \<Longrightarrow>
+   \<Gamma> \<turnstile> Call src\<^sub>1 SafeArrowCall call\<^sub>1 \<Rrightarrow>
+    Call (OperationCall src\<^sub>2 ArrowCall ExcludingOp [NullLiteral])
+      ArrowCall call\<^sub>2"
 |CollectionDotCallN:
-  "\<Gamma> \<turnstile> src1 \<Rrightarrow> src2 \<Longrightarrow>
-   \<Gamma> \<turnstile> src2 : \<tau> \<Longrightarrow>
+  "\<Gamma> \<turnstile> src\<^sub>1 \<Rrightarrow> src\<^sub>2 \<Longrightarrow>
+   \<Gamma> \<turnstile> src\<^sub>2 : \<tau> \<Longrightarrow>
    element_type \<tau> \<sigma> \<Longrightarrow>
    \<not> OclVoid[?] \<le> \<sigma> \<Longrightarrow>
-   (\<Gamma>, \<tau>) \<turnstile>\<^sub>C call1 \<Rrightarrow> call2 \<Longrightarrow>
+   (\<Gamma>, \<tau>) \<turnstile>\<^sub>C call\<^sub>1 \<Rrightarrow> call\<^sub>2 \<Longrightarrow>
    it = new_vname \<Gamma> \<Longrightarrow>
-   \<Gamma> \<turnstile> Call src1 DotCall call1 \<Rrightarrow> CollectIteratorCall src2 [it]
-          (Call (Var it) DotCall call2)"
+   \<Gamma> \<turnstile> Call src\<^sub>1 DotCall call\<^sub>1 \<Rrightarrow> CollectIteratorCall src\<^sub>2 [it]
+          (Call (Var it) DotCall call\<^sub>2)"
 |CollectionSafeDotCallN:
-  "\<Gamma> \<turnstile> src1 \<Rrightarrow> src2 \<Longrightarrow>
-   \<Gamma> \<turnstile> src2 : \<tau> \<Longrightarrow>
+  "\<Gamma> \<turnstile> src\<^sub>1 \<Rrightarrow> src\<^sub>2 \<Longrightarrow>
+   \<Gamma> \<turnstile> src\<^sub>2 : \<tau> \<Longrightarrow>
    element_type \<tau> \<sigma> \<Longrightarrow>
    OclVoid[?] \<le> \<sigma> \<Longrightarrow>
-   (\<Gamma>, \<tau>) \<turnstile>\<^sub>C call1 \<Rrightarrow> call2 \<Longrightarrow>
+   (\<Gamma>, \<tau>) \<turnstile>\<^sub>C call\<^sub>1 \<Rrightarrow> call\<^sub>2 \<Longrightarrow>
    it = new_vname \<Gamma> \<Longrightarrow>
-   \<Gamma> \<turnstile> Call src1 SafeDotCall call1 \<Rrightarrow>
-      CollectIteratorCall (OperationCall src2 ArrowCall ExcludingOp [NullLiteral])
-        [it] (Call (Var it) DotCall call2)"
+   \<Gamma> \<turnstile> Call src\<^sub>1 SafeDotCall call\<^sub>1 \<Rrightarrow>
+      CollectIteratorCall (OperationCall src\<^sub>2 ArrowCall ExcludingOp [NullLiteral])
+        [it] (Call (Var it) DotCall call\<^sub>2)"
 
 |TypeOperationN:
   "(\<Gamma>, \<tau>) \<turnstile>\<^sub>C TypeOperation op ty \<Rrightarrow> TypeOperation op ty"
@@ -150,15 +150,15 @@ inductive normalize
 
 |IterateN:
   "element_type \<tau> \<sigma> \<Longrightarrow>
-   \<Gamma> \<turnstile> res_init1 \<Rrightarrow> res_init2 \<Longrightarrow>
+   \<Gamma> \<turnstile> res_init\<^sub>1 \<Rrightarrow> res_init\<^sub>2 \<Longrightarrow>
    fmadd \<Gamma> (fmap_of_list (map (\<lambda>it. (it, \<sigma>)) its)) \<turnstile>
-      Let res res_t res_init1 body1 \<Rrightarrow> Let res res_t res_init2 body2 \<Longrightarrow>
-   (\<Gamma>, \<tau>) \<turnstile>\<^sub>C Iterate its res res_t res_init1 body1 \<Rrightarrow>
-      Iterate its res res_t res_init2 body2"
+      Let res res_t res_init\<^sub>1 body\<^sub>1 \<Rrightarrow> Let res res_t res_init\<^sub>2 body\<^sub>2 \<Longrightarrow>
+   (\<Gamma>, \<tau>) \<turnstile>\<^sub>C Iterate its res res_t res_init\<^sub>1 body\<^sub>1 \<Rrightarrow>
+      Iterate its res res_t res_init\<^sub>2 body\<^sub>2"
 |IteratorN:
   "element_type \<tau> \<sigma> \<Longrightarrow>
-   fmadd \<Gamma> (fmap_of_list (map (\<lambda>it. (it, \<sigma>)) its)) \<turnstile> body1 \<Rrightarrow> body2  \<Longrightarrow>
-   (\<Gamma>, \<tau>) \<turnstile>\<^sub>C Iterator iter its body1 \<Rrightarrow> Iterator iter its body2"
+   fmadd \<Gamma> (fmap_of_list (map (\<lambda>it. (it, \<sigma>)) its)) \<turnstile> body\<^sub>1 \<Rrightarrow> body\<^sub>2  \<Longrightarrow>
+   (\<Gamma>, \<tau>) \<turnstile>\<^sub>C Iterator iter its body\<^sub>1 \<Rrightarrow> Iterator iter its body\<^sub>2"
 
 |ExprListNilN:
   "\<Gamma> \<turnstile>\<^sub>L [] \<Rrightarrow> []"
@@ -179,9 +179,9 @@ inductive_cases ArrowCallNE [elim]: "\<Gamma> \<turnstile> Call src ArrowCall ca
 inductive_cases SafeArrowCallNE [elim]: "\<Gamma> \<turnstile> Call src SafeArrowCall call \<Rrightarrow> b"
 
 inductive_cases CallNE [elim]: "(\<Gamma>, \<tau>) \<turnstile>\<^sub>C call \<Rrightarrow> b"
-inductive_cases OperationCallNE [elim]: "(\<Gamma>, \<tau>) \<turnstile>\<^sub>C Operation op as \<Rrightarrow> call2"
-inductive_cases IterateCallNE [elim]: "(\<Gamma>, \<tau>) \<turnstile>\<^sub>C Iterate its res res_t res_init1 body1 \<Rrightarrow> call2"
-inductive_cases IteratorCallNE [elim]: "(\<Gamma>, \<tau>) \<turnstile>\<^sub>C Iterator iter its body1 \<Rrightarrow> call2"
+inductive_cases OperationCallNE [elim]: "(\<Gamma>, \<tau>) \<turnstile>\<^sub>C Operation op as \<Rrightarrow> call"
+inductive_cases IterateCallNE [elim]: "(\<Gamma>, \<tau>) \<turnstile>\<^sub>C Iterate its res res_t res_init body \<Rrightarrow> call"
+inductive_cases IteratorCallNE [elim]: "(\<Gamma>, \<tau>) \<turnstile>\<^sub>C Iterator iter its body \<Rrightarrow> call"
 
 inductive_cases ExprListNilNE [elim]: "\<Gamma> \<turnstile>\<^sub>L x # xs \<Rrightarrow> zs"
 
@@ -190,25 +190,28 @@ inductive_cases ExprListNilNE [elim]: "\<Gamma> \<turnstile>\<^sub>L x # xs \<Rr
 section \<open>Determinism\<close>
 
 lemma any_has_not_element_type:
-  "\<tau> \<le> OclAny[?] \<Longrightarrow> element_type \<tau> \<sigma> \<Longrightarrow> False"
+  "element_type \<tau> \<sigma> \<Longrightarrow> \<tau> \<le> OclAny[?] \<Longrightarrow> False"
   by (erule element_type.cases; auto)
 
 lemma any_has_not_element_type':
-  "\<tau> \<le> OclAny[1] \<or> \<tau> \<le> Tuple fmempty \<Longrightarrow> element_type \<tau> \<sigma> \<Longrightarrow> False"
+  "element_type \<tau> \<sigma> \<Longrightarrow> \<tau> \<le> OclAny[1] \<or> \<tau> \<le> Tuple fmempty \<Longrightarrow> False"
   by (erule element_type.cases; auto)
 
 lemma any_has_not_element_type'':
-  "\<tau> \<le> OclAny[?] \<or> \<tau> \<le> Tuple fmempty \<Longrightarrow> element_type \<tau> \<sigma> \<Longrightarrow> False"
+  "element_type \<tau> \<sigma> \<Longrightarrow> \<tau> \<le> OclAny[?] \<or> \<tau> \<le> Tuple fmempty \<Longrightarrow> False"
   by (erule element_type.cases; auto)
 
 lemma any_has_not_element_type''':
-  "OclVoid[?] \<le> \<tau> \<Longrightarrow> element_type \<tau> \<sigma> \<Longrightarrow> False"
+  "element_type \<tau> \<sigma> \<Longrightarrow> OclVoid[?] \<le> \<tau> \<Longrightarrow> False"
   by (erule element_type.cases; auto)
 
 lemma
-  normalize_det: "\<Gamma> \<turnstile> expr \<Rrightarrow> expr\<^sub>1 \<Longrightarrow> \<Gamma> \<turnstile> expr \<Rrightarrow> expr\<^sub>2 \<Longrightarrow> expr\<^sub>1 = expr\<^sub>2" and
-  normalize_call_det: "\<Gamma>_\<tau> \<turnstile>\<^sub>C call \<Rrightarrow> call\<^sub>1 \<Longrightarrow> \<Gamma>_\<tau> \<turnstile>\<^sub>C call \<Rrightarrow> call\<^sub>2 \<Longrightarrow> call\<^sub>1 = call\<^sub>2" and
-  normalize_expr_list_det: "\<Gamma> \<turnstile>\<^sub>L xs \<Rrightarrow> ys \<Longrightarrow> \<Gamma> \<turnstile>\<^sub>L xs \<Rrightarrow> zs \<Longrightarrow> ys = zs"
+  normalize_det:
+    "\<Gamma> \<turnstile> expr \<Rrightarrow> expr\<^sub>1 \<Longrightarrow> \<Gamma> \<turnstile> expr \<Rrightarrow> expr\<^sub>2 \<Longrightarrow> expr\<^sub>1 = expr\<^sub>2" and
+  normalize_call_det:
+    "\<Gamma>_\<tau> \<turnstile>\<^sub>C call \<Rrightarrow> call\<^sub>1 \<Longrightarrow> \<Gamma>_\<tau> \<turnstile>\<^sub>C call \<Rrightarrow> call\<^sub>2 \<Longrightarrow> call\<^sub>1 = call\<^sub>2" and
+  normalize_expr_list_det:
+    "\<Gamma> \<turnstile>\<^sub>L xs \<Rrightarrow> ys \<Longrightarrow> \<Gamma> \<turnstile>\<^sub>L xs \<Rrightarrow> zs \<Longrightarrow> ys = zs"
   for \<Gamma> :: "('a :: ocl_object_model) type env"
   and \<Gamma>_\<tau> :: "('a :: ocl_object_model) type env \<times> 'a type"
 proof (induct \<Gamma> expr expr\<^sub>1 and \<Gamma>_\<tau> call call\<^sub>1
@@ -216,73 +219,64 @@ proof (induct \<Gamma> expr expr\<^sub>1 and \<Gamma>_\<tau> call call\<^sub>1
        rule: normalize_normalize_call_normalize_expr_list.inducts)
   case (LiteralN \<Gamma> a) thus ?case by auto
 next
-  case (LetN \<Gamma> init1 init2 v \<tau> body1 body2) thus ?case by blast
+  case (LetN \<Gamma> init\<^sub>1 init\<^sub>2 v \<tau> body\<^sub>1 body\<^sub>2) thus ?case by blast
 next
   case (VarN \<Gamma> v) thus ?case by auto
 next
-  case (IfN \<Gamma> a1 a2 b1 b2 c1 c2) thus ?case
+  case (IfN \<Gamma> a\<^sub>1 a\<^sub>2 b\<^sub>1 b\<^sub>2 c\<^sub>1 c\<^sub>2) thus ?case
     apply (insert IfN.prems)
     apply (erule IfNE)
-    by (simp add: IfN.hyps(2) IfN.hyps(4) IfN.hyps(6))
+    by (simp add: IfN.hyps)
 next
   case (MetaOperationCallN \<Gamma> \<tau> op) thus ?case by auto
 next
   case (StaticOperationCallN \<Gamma> as bs \<tau> op) thus ?case by blast
 next
-  case (OclAnyDotCallN \<Gamma> src1 src2 \<tau> call1 call2) show ?case
+  case (OclAnyDotCallN \<Gamma> src\<^sub>1 src\<^sub>2 \<tau> call\<^sub>1 call\<^sub>2) show ?case
     apply (insert OclAnyDotCallN.prems)
     apply (erule DotCallNE)
-    apply (metis OclAnyDotCallN.hyps(2) OclAnyDotCallN.hyps(3) OclAnyDotCallN.hyps(6) typing_det)
-    by (metis OclAnyDotCallN.hyps(2) OclAnyDotCallN.hyps(3) OclAnyDotCallN.hyps(4) any_has_not_element_type' typing_det)
+    using OclAnyDotCallN.hyps typing_det apply metis
+    using OclAnyDotCallN.hyps any_has_not_element_type' typing_det by metis
 next
-  case (OclAnySafeDotCallN \<Gamma> src1 src2 \<tau> call1 call2) show ?case
+  case (OclAnySafeDotCallN \<Gamma> src\<^sub>1 src\<^sub>2 \<tau> call\<^sub>1 call\<^sub>2) show ?case
     apply (insert OclAnySafeDotCallN.prems)
     apply (erule SafeDotCallNE)
-    apply (metis (no_types, lifting) OclAnySafeDotCallN.hyps(2) OclAnySafeDotCallN.hyps(3) OclAnySafeDotCallN.hyps(6) comp_apply list.simps(8) list.simps(9) typing_det)
-    by (metis OclAnySafeDotCallN.hyps(2) OclAnySafeDotCallN.hyps(3) OclAnySafeDotCallN.hyps(4) any_has_not_element_type''' typing_det)
+    using OclAnySafeDotCallN.hyps typing_det comp_apply
+    apply (metis (no_types, lifting) list.simps(8) list.simps(9))
+    using OclAnySafeDotCallN.hyps typing_det any_has_not_element_type''' by metis
 next
-  case (OclAnyArrowDotCallN \<Gamma> src1 src2 \<tau> call1 call2) show ?case
+  case (OclAnyArrowDotCallN \<Gamma> src\<^sub>1 src\<^sub>2 \<tau> call\<^sub>1 call\<^sub>2) show ?case
     apply (insert OclAnyArrowDotCallN.prems)
     apply (erule ArrowCallNE)
-    apply (metis OclAnyArrowDotCallN.hyps(2) OclAnyArrowDotCallN.hyps(3) OclAnyArrowDotCallN.hyps(6) comp_apply typing_det)
-    by (metis OclAnyArrowDotCallN.hyps(2) OclAnyArrowDotCallN.hyps(3) OclAnyArrowDotCallN.hyps(4) any_has_not_element_type'' typing_det)
+    using OclAnyArrowDotCallN.hyps typing_det comp_apply apply metis
+    using OclAnyArrowDotCallN.hyps typing_det any_has_not_element_type'' by metis
 next
-  case (CollectionArrowCallN \<Gamma> src1 src2 \<tau> call1 call2 uu) show ?case
+  case (CollectionArrowCallN \<Gamma> src\<^sub>1 src\<^sub>2 \<tau> call\<^sub>1 call\<^sub>2 uu) show ?case
     apply (insert CollectionArrowCallN.prems)
     apply (erule ArrowCallNE)
-    apply (metis CollectionArrowCallN.hyps(2) CollectionArrowCallN.hyps(3) CollectionArrowCallN.hyps(4) any_has_not_element_type'' typing_det)
-    using CollectionArrowCallN.hyps(2) CollectionArrowCallN.hyps(3) CollectionArrowCallN.hyps(6) typing_det by fastforce
+    using CollectionArrowCallN.hyps typing_det any_has_not_element_type'' apply metis
+    using CollectionArrowCallN.hyps typing_det by metis
 next
-  case (CollectionSafeArrowCallN \<Gamma> src1 src2 \<tau> call1 call2 \<sigma>) show ?case
+  case (CollectionSafeArrowCallN \<Gamma> src\<^sub>1 src\<^sub>2 \<tau> call\<^sub>1 call\<^sub>2 \<sigma>) show ?case
     apply (insert CollectionSafeArrowCallN.prems)
     apply (erule SafeArrowCallNE)
-    by (smt CollectionSafeArrowCallN.hyps(2) CollectionSafeArrowCallN.hyps(3) CollectionSafeArrowCallN.hyps(7) comp_assoc comp_eq_dest_lhs list.simps(8) list.simps(9) typing_det)
+    using CollectionSafeArrowCallN.hyps typing_det comp_apply
+    by (metis (no_types, lifting) list.simps(8) list.simps(9))
 next
-  case (CollectionDotCallN \<Gamma> src1 src2 \<tau> call1 call2 \<sigma> it) show ?case
+  case (CollectionDotCallN \<Gamma> src\<^sub>1 src\<^sub>2 \<tau> call\<^sub>1 call\<^sub>2 \<sigma> it) show ?case
     apply (insert CollectionDotCallN.prems)
     apply (erule DotCallNE)
-    apply (metis CollectionDotCallN.hyps(2) CollectionDotCallN.hyps(3) CollectionDotCallN.hyps(4) any_has_not_element_type' typing_det)
-    using CollectionDotCallN.hyps(2) CollectionDotCallN.hyps(3) CollectionDotCallN.hyps(7) CollectionDotCallN.hyps(8) typing_det by fastforce
+    using CollectionDotCallN.hyps typing_det any_has_not_element_type' apply metis
+    using CollectionDotCallN.hyps typing_det by metis
 next
-  case (CollectionSafeDotCallN \<Gamma> src1 src2 \<tau> call1 call2 \<sigma> it) show ?case
+  case (CollectionSafeDotCallN \<Gamma> src\<^sub>1 src\<^sub>2 \<tau> call\<^sub>1 call\<^sub>2 \<sigma> it) show ?case
     apply (insert CollectionSafeDotCallN.prems)
     apply (erule SafeDotCallNE)
-    apply (metis CollectionSafeDotCallN.hyps(2) CollectionSafeDotCallN.hyps(3) CollectionSafeDotCallN.hyps(4) any_has_not_element_type''' typing_det)
-    by (metis (no_types, lifting) CollectionSafeDotCallN.hyps(2) CollectionSafeDotCallN.hyps(3) CollectionSafeDotCallN.hyps(7) CollectionSafeDotCallN.hyps(8) comp_apply list.simps(8) list.simps(9) typing_det)
+    using CollectionSafeDotCallN.hyps typing_det any_has_not_element_type''' apply metis
+    using CollectionSafeDotCallN.hyps typing_det comp_apply
+    by (metis (no_types, lifting) list.simps(8) list.simps(9))
 next
   case (TypeOperationN \<Gamma> \<tau> op ty) thus ?case by auto
-next
-  case (IterateN \<tau> \<sigma> \<Gamma> res_init1 res_init2 its res res_t body1 body2)
-  show ?case
-    apply (insert IterateN.prems)
-    apply (erule IterateCallNE)
-    using IterateN.hyps(1) IterateN.hyps(5) element_type_det by blast
-next
-  case (IteratorN \<tau> \<sigma> \<Gamma> its body1 body2 iter)
-  show ?case
-    apply (insert IteratorN.prems)
-    apply (erule IteratorCallNE)
-    using IteratorN.hyps(1) IteratorN.hyps(3) element_type_det by auto
 next
   case (AttributeN \<Gamma> \<tau> attr) thus ?case by auto
 next
@@ -291,9 +285,21 @@ next
   case (OperationN \<Gamma> as bs \<tau> op) show ?case
     apply (insert OperationN.prems)
     apply (erule OperationCallNE)
-    by (simp add: OperationN.hyps(2))
+    by (simp add: OperationN.hyps)
 next
   case (TupleElementN \<Gamma> \<tau> elem) thus ?case by auto
+next
+  case (IterateN \<tau> \<sigma> \<Gamma> res_init\<^sub>1 res_init\<^sub>2 its res res_t body\<^sub>1 body\<^sub>2)
+  show ?case
+    apply (insert IterateN.prems)
+    apply (erule IterateCallNE)
+    using IterateN.hyps element_type_det by blast
+next
+  case (IteratorN \<tau> \<sigma> \<Gamma> its body\<^sub>1 body\<^sub>2 iter)
+  show ?case
+    apply (insert IteratorN.prems)
+    apply (erule IteratorCallNE)
+    using IteratorN.hyps element_type_det by blast
 next
   case (ExprListNilN \<Gamma>) thus ?case
     using normalize_expr_list.cases by auto
