OCL_Basic_Types.thy
@@ -16,15 +16,15 @@ type_synonym 'a enum = "('a, String.literal) phantom"
 type_synonym elit = String.literal
 
 datatype ('a :: order) basic_type =
-  OclVoid
+  OclAny
+| OclVoid
 | Boolean
-| UnlimitedNatural
-| Integer
 | Real
+| Integer
+| UnlimitedNatural
 | String
 | ObjectType 'a ("\<langle>_\<rangle>\<^sub>\<T>" [0] 1000)
 | Enum "'a enum"
-| OclAny
 
 inductive basic_subtype ("_ \<sqsubset>\<^sub>B _" [65, 65] 65) where
   "OclVoid \<sqsubset>\<^sub>B Boolean"
@@ -45,18 +45,18 @@ inductive basic_subtype ("_ \<sqsubset>\<^sub>B _" [65, 65] 65) where
 
 declare basic_subtype.intros [intro!]
 
+inductive_cases basic_subtype_x_OclAny [elim!]: "\<tau> \<sqsubset>\<^sub>B OclAny"
 inductive_cases basic_subtype_x_OclVoid [elim!]: "\<tau> \<sqsubset>\<^sub>B OclVoid"
 inductive_cases basic_subtype_x_Boolean [elim!]: "\<tau> \<sqsubset>\<^sub>B Boolean"
-inductive_cases basic_subtype_x_UnlimitedNatural [elim!]: "\<tau> \<sqsubset>\<^sub>B UnlimitedNatural"
-inductive_cases basic_subtype_x_Integer [elim!]: "\<tau> \<sqsubset>\<^sub>B Integer"
 inductive_cases basic_subtype_x_Real [elim!]: "\<tau> \<sqsubset>\<^sub>B Real"
+inductive_cases basic_subtype_x_Integer [elim!]: "\<tau> \<sqsubset>\<^sub>B Integer"
+inductive_cases basic_subtype_x_UnlimitedNatural [elim!]: "\<tau> \<sqsubset>\<^sub>B UnlimitedNatural"
 inductive_cases basic_subtype_x_String [elim!]: "\<tau> \<sqsubset>\<^sub>B String"
 inductive_cases basic_subtype_x_ObjectType [elim!]: "\<tau> \<sqsubset>\<^sub>B \<langle>\<C>\<rangle>\<^sub>\<T>"
 inductive_cases basic_subtype_x_Enum [elim!]: "\<tau> \<sqsubset>\<^sub>B Enum \<E>"
-inductive_cases basic_subtype_x_OclAny [elim!]: "\<tau> \<sqsubset>\<^sub>B OclAny"
 
-inductive_cases basic_subtype_ObjectType_x [elim!]: "\<langle>\<C>\<rangle>\<^sub>\<T> \<sqsubset>\<^sub>B \<sigma>"
 inductive_cases basic_subtype_OclAny_x [elim!]: "OclAny \<sqsubset>\<^sub>B \<sigma>"
+inductive_cases basic_subtype_ObjectType_x [elim!]: "\<langle>\<C>\<rangle>\<^sub>\<T> \<sqsubset>\<^sub>B \<sigma>"
 
 lemma basic_subtype_asym:
   "\<tau> \<sqsubset>\<^sub>B \<sigma> \<Longrightarrow> \<sigma> \<sqsubset>\<^sub>B \<tau> \<Longrightarrow> False"
@@ -76,37 +76,33 @@ definition "(\<le>) \<equiv> basic_subtype\<^sup>*\<^sup>*"
 
 subsection \<open>Introduction Rules\<close>
 
+lemma type_less_eq_x_OclAny_intro [intro]:
+  "\<tau> \<le> OclAny"
+proof -
+  have "basic_subtype\<^sup>*\<^sup>* OclVoid OclAny"
+    by (rule_tac ?b="Boolean" in rtranclp.rtrancl_into_rtrancl; auto)
+  moreover have "basic_subtype\<^sup>*\<^sup>* Integer OclAny"
+    by (rule_tac ?b="Real" in rtranclp.rtrancl_into_rtrancl; auto)
+  moreover hence "basic_subtype\<^sup>*\<^sup>* UnlimitedNatural OclAny"
+    by (rule_tac ?b="Integer" in converse_rtranclp_into_rtranclp; auto)
+  ultimately show ?thesis
+    unfolding less_eq_basic_type_def
+    by (induct \<tau>; auto)
+qed
+
 lemma type_less_eq_OclVoid_x_intro [intro]:
   "OclVoid \<le> \<tau>"
-  unfolding less_eq_basic_type_def
-proof (induct \<tau>)
-  case OclVoid thus ?case by simp
-next
-  case Boolean thus ?case by auto
-next
-  case UnlimitedNatural thus ?case by auto
-next
-  case Integer
-  have "basic_subtype\<^sup>*\<^sup>* OclVoid UnlimitedNatural" by auto
-  also have "basic_subtype\<^sup>*\<^sup>* UnlimitedNatural Integer" by auto
-  finally show ?case by auto
-next
-  case Real
-  have "basic_subtype\<^sup>*\<^sup>* OclVoid UnlimitedNatural" by auto
-  also have "basic_subtype\<^sup>*\<^sup>* UnlimitedNatural Integer" by auto
-  also have "basic_subtype\<^sup>*\<^sup>* Integer Real" by auto
-  finally show ?case by auto
-next
-  case String thus ?case by auto
-next
-  case (ObjectType x) thus ?case by auto
-next
-  case (Enum x) thus ?case by auto
-next
-  case OclAny
-  have "basic_subtype\<^sup>*\<^sup>* OclVoid Boolean" by auto
-  also have "basic_subtype\<^sup>*\<^sup>* Boolean OclAny" by auto
-  finally show ?case by auto
+proof -
+  have "basic_subtype\<^sup>*\<^sup>* OclVoid OclAny"
+    by (metis (mono_tags) OCL_Basic_Types.less_eq_basic_type_def
+          OCL_Basic_Types.type_less_eq_x_OclAny_intro)
+  moreover have "basic_subtype\<^sup>*\<^sup>* OclVoid Integer"
+    by (rule_tac ?b="UnlimitedNatural" in rtranclp.rtrancl_into_rtrancl; auto)
+  moreover hence "basic_subtype\<^sup>*\<^sup>* OclVoid Real"
+    by (rule_tac ?b="Integer" in rtranclp.rtrancl_into_rtrancl; auto)
+  ultimately show ?thesis
+    unfolding less_eq_basic_type_def
+    by (induct \<tau>; auto)
 qed
 
 lemma type_less_eq_x_Real_intro [intro]:
@@ -125,24 +121,35 @@ lemma type_less_eq_x_ObjectType_intro [intro]:
   unfolding less_eq_basic_type_def
   using dual_order.order_iff_strict by blast
 
-lemma type_less_eq_x_OclAny_intro [intro]:
-  "\<tau> \<le> OclAny"
-proof -
-  have "basic_subtype\<^sup>*\<^sup>* OclVoid OclAny"
-    by (metis (mono_tags) OCL_Basic_Types.less_eq_basic_type_def
-        OCL_Basic_Types.type_less_eq_OclVoid_x_intro)
-  moreover have "basic_subtype\<^sup>*\<^sup>* Integer OclAny"
-    by (rule_tac ?b="Real" in rtranclp.rtrancl_into_rtrancl; auto)
-  moreover hence "basic_subtype\<^sup>*\<^sup>* UnlimitedNatural OclAny"
-    by (rule_tac ?b="Integer" in converse_rtranclp_into_rtranclp; auto)
-  ultimately show ?thesis
-    unfolding less_eq_basic_type_def
-    by (induct \<tau>, auto)
-qed
-
 (*** Elimination Rules ******************************************************)
 
 subsection \<open>Elimination Rules\<close>
+
+lemma type_less_x_OclAny [elim!]:
+  "\<tau> < OclAny \<Longrightarrow>
+   (\<tau> = OclVoid \<Longrightarrow> P) \<Longrightarrow>
+   (\<tau> = Boolean \<Longrightarrow> P) \<Longrightarrow>
+   (\<tau> = Integer \<Longrightarrow> P) \<Longrightarrow>
+   (\<tau> = UnlimitedNatural \<Longrightarrow> P) \<Longrightarrow>
+   (\<tau> = Real \<Longrightarrow> P) \<Longrightarrow>
+   (\<tau> = String \<Longrightarrow> P) \<Longrightarrow>
+   (\<And>\<E>. \<tau> = Enum \<E> \<Longrightarrow> P) \<Longrightarrow> 
+   (\<And>\<C>. \<tau> = \<langle>\<C>\<rangle>\<^sub>\<T> \<Longrightarrow> P) \<Longrightarrow> P"
+  unfolding less_basic_type_def
+  by (induct rule: converse_tranclp_induct; auto)
+
+lemma type_less_eq_x_OclAny [elim!]:
+  "\<tau> \<le> OclAny \<Longrightarrow>
+   (\<tau> = OclVoid \<Longrightarrow> P) \<Longrightarrow>
+   (\<tau> = OclAny \<Longrightarrow> P) \<Longrightarrow>
+   (\<tau> = Boolean \<Longrightarrow> P) \<Longrightarrow>
+   (\<tau> = Integer \<Longrightarrow> P) \<Longrightarrow>
+   (\<tau> = UnlimitedNatural \<Longrightarrow> P) \<Longrightarrow>
+   (\<tau> = Real \<Longrightarrow> P) \<Longrightarrow>
+   (\<tau> = String \<Longrightarrow> P) \<Longrightarrow>
+   (\<And>\<E>. \<tau> = Enum \<E> \<Longrightarrow> P) \<Longrightarrow> 
+   (\<And>\<C>. \<tau> = \<langle>\<C>\<rangle>\<^sub>\<T> \<Longrightarrow> P) \<Longrightarrow> P"
+  by (erule basic_type.exhaust; auto)
 
 lemma type_less_x_OclVoid [elim!]:
   "\<tau> < OclVoid \<Longrightarrow> P"
@@ -168,16 +175,20 @@ lemma type_less_eq_x_Boolean [elim!]:
   unfolding less_eq_basic_type_def
   by (induct rule: converse_rtranclp_induct; auto)
 
-lemma type_less_x_UnlimitedNatural [elim!]:
-  "\<tau> < UnlimitedNatural \<Longrightarrow>
-   (\<tau> = OclVoid \<Longrightarrow> P) \<Longrightarrow> P"
+lemma type_less_x_Real [elim!]:
+  "\<tau> < Real \<Longrightarrow>
+   (\<tau> = OclVoid \<Longrightarrow> P) \<Longrightarrow>
+   (\<tau> = UnlimitedNatural \<Longrightarrow> P) \<Longrightarrow>
+   (\<tau> = Integer \<Longrightarrow> P) \<Longrightarrow> P"
   unfolding less_basic_type_def
   by (induct rule: converse_tranclp_induct; auto)
 
-lemma type_less_eq_x_UnlimitedNatural [elim!]:
-  "\<tau> \<le> UnlimitedNatural \<Longrightarrow>
+lemma type_less_eq_x_Real [elim!]:
+  "\<tau> \<le> Real \<Longrightarrow>
    (\<tau> = OclVoid \<Longrightarrow> P) \<Longrightarrow>
-   (\<tau> = UnlimitedNatural \<Longrightarrow> P) \<Longrightarrow> P"
+   (\<tau> = UnlimitedNatural \<Longrightarrow> P) \<Longrightarrow>
+   (\<tau> = Integer \<Longrightarrow> P) \<Longrightarrow>
+   (\<tau> = Real \<Longrightarrow> P) \<Longrightarrow> P"
   unfolding less_eq_basic_type_def
   by (induct rule: converse_rtranclp_induct; auto)
 
@@ -196,20 +207,16 @@ lemma type_less_eq_x_Integer [elim!]:
   unfolding less_eq_basic_type_def
   by (induct rule: converse_rtranclp_induct; auto)
 
-lemma type_less_x_Real [elim!]:
-  "\<tau> < Real \<Longrightarrow>
-   (\<tau> = OclVoid \<Longrightarrow> P) \<Longrightarrow>
-   (\<tau> = UnlimitedNatural \<Longrightarrow> P) \<Longrightarrow>
-   (\<tau> = Integer \<Longrightarrow> P) \<Longrightarrow> P"
+lemma type_less_x_UnlimitedNatural [elim!]:
+  "\<tau> < UnlimitedNatural \<Longrightarrow>
+   (\<tau> = OclVoid \<Longrightarrow> P) \<Longrightarrow> P"
   unfolding less_basic_type_def
   by (induct rule: converse_tranclp_induct; auto)
 
-lemma type_less_eq_x_Real [elim!]:
-  "\<tau> \<le> Real \<Longrightarrow>
+lemma type_less_eq_x_UnlimitedNatural [elim!]:
+  "\<tau> \<le> UnlimitedNatural \<Longrightarrow>
    (\<tau> = OclVoid \<Longrightarrow> P) \<Longrightarrow>
-   (\<tau> = UnlimitedNatural \<Longrightarrow> P) \<Longrightarrow>
-   (\<tau> = Integer \<Longrightarrow> P) \<Longrightarrow>
-   (\<tau> = Real \<Longrightarrow> P) \<Longrightarrow> P"
+   (\<tau> = UnlimitedNatural \<Longrightarrow> P) \<Longrightarrow> P"
   unfolding less_eq_basic_type_def
   by (induct rule: converse_rtranclp_induct; auto)
 
@@ -256,32 +263,6 @@ lemma type_less_eq_x_Enum [elim!]:
    (\<tau> = Enum \<E> \<Longrightarrow> P) \<Longrightarrow> P"
   unfolding less_eq_basic_type_def
   by (induct rule: converse_rtranclp_induct; auto)
-
-lemma type_less_x_OclAny [elim!]:
-  "\<tau> < OclAny \<Longrightarrow>
-   (\<tau> = OclVoid \<Longrightarrow> P) \<Longrightarrow>
-   (\<tau> = Boolean \<Longrightarrow> P) \<Longrightarrow>
-   (\<tau> = Integer \<Longrightarrow> P) \<Longrightarrow>
-   (\<tau> = UnlimitedNatural \<Longrightarrow> P) \<Longrightarrow>
-   (\<tau> = Real \<Longrightarrow> P) \<Longrightarrow>
-   (\<tau> = String \<Longrightarrow> P) \<Longrightarrow>
-   (\<And>\<E>. \<tau> = Enum \<E> \<Longrightarrow> P) \<Longrightarrow> 
-   (\<And>\<C>. \<tau> = \<langle>\<C>\<rangle>\<^sub>\<T> \<Longrightarrow> P) \<Longrightarrow> P"
-  unfolding less_basic_type_def
-  by (induct rule: converse_tranclp_induct; auto)
-
-lemma type_less_eq_x_OclAny [elim!]:
-  "\<tau> \<le> OclAny \<Longrightarrow>
-   (\<tau> = OclVoid \<Longrightarrow> P) \<Longrightarrow>
-   (\<tau> = OclAny \<Longrightarrow> P) \<Longrightarrow>
-   (\<tau> = Boolean \<Longrightarrow> P) \<Longrightarrow>
-   (\<tau> = Integer \<Longrightarrow> P) \<Longrightarrow>
-   (\<tau> = UnlimitedNatural \<Longrightarrow> P) \<Longrightarrow>
-   (\<tau> = Real \<Longrightarrow> P) \<Longrightarrow>
-   (\<tau> = String \<Longrightarrow> P) \<Longrightarrow>
-   (\<And>\<E>. \<tau> = Enum \<E> \<Longrightarrow> P) \<Longrightarrow> 
-   (\<And>\<C>. \<tau> = \<langle>\<C>\<rangle>\<^sub>\<T> \<Longrightarrow> P) \<Longrightarrow> P"
-  by (erule basic_type.exhaust; auto)
 
 (*** Properties *************************************************************)
 
@@ -378,18 +359,18 @@ section \<open>Code Setup\<close>
 code_pred basic_subtype .
 
 fun basic_subtype_fun :: "'a::order basic_type \<Rightarrow> 'a basic_type \<Rightarrow> bool" where
-  "basic_subtype_fun OclVoid \<sigma> = (\<sigma> \<noteq> OclVoid)"
+  "basic_subtype_fun OclAny _ = False"
+| "basic_subtype_fun OclVoid \<sigma> = (\<sigma> \<noteq> OclVoid)"
 | "basic_subtype_fun Boolean \<sigma> = (\<sigma> = OclAny)"
-| "basic_subtype_fun UnlimitedNatural \<sigma> = (\<sigma> = Integer \<or> \<sigma> = Real \<or> \<sigma> = OclAny)"
-| "basic_subtype_fun Integer \<sigma> = (\<sigma> = Real \<or> \<sigma> = OclAny)"
 | "basic_subtype_fun Real \<sigma> = (\<sigma> = OclAny)"
+| "basic_subtype_fun Integer \<sigma> = (\<sigma> = Real \<or> \<sigma> = OclAny)"
+| "basic_subtype_fun UnlimitedNatural \<sigma> = (\<sigma> = Integer \<or> \<sigma> = Real \<or> \<sigma> = OclAny)"
 | "basic_subtype_fun String \<sigma> = (\<sigma> = OclAny)"
 | "basic_subtype_fun \<langle>\<C>\<rangle>\<^sub>\<T> \<sigma> = (case \<sigma>
     of \<langle>\<D>\<rangle>\<^sub>\<T> \<Rightarrow> \<C> < \<D>
      | OclAny \<Rightarrow> True
      | _ \<Rightarrow> False)"
 | "basic_subtype_fun (Enum _) \<sigma> = (\<sigma> = OclAny)"
-| "basic_subtype_fun OclAny _ = False"
 
 lemma less_eq_basic_type_code [code_abbrev, simp]:
   "\<tau> = \<sigma> \<or> basic_subtype_fun \<tau> \<sigma> \<longleftrightarrow> \<tau> \<le> \<sigma>"
